theories/algebra/view.v
@@ -16,36 +16,19 @@ Notation viewUR := (gmapUR loc max_natUR).
 
 Implicit Types (V W : view) (ℓ : loc).
 
-(* Definition maybe_max mx my :=
-  match mx, my withtime
-  | Some x, Some y => Some (x `max` y)
-  | _, _ => None end). *)
-
 Instance join_view : Join view :=
   λ a b, a ⋅ b.
-  (* (merge (λ (x1 x2 : nat), Some (x1 `max` x2))). *)
-
-(* Instance join_view : Join view := (union_with (λ (x1 x2 : nat), Some (x1 `max` x2))). *)
 
 Instance subseteq_view : SqSubsetEq view := λ v w, v ≼ w.
-  (* λ v w, v ⊔ w = w. *)
-  (* λ v w, ∀ k t, v !! k = Some t → ∃ t', w !! k = Some t' ∧ t ≤ t'. *)
+
+Lemma view_join V W : (V ⊔ W) = (V ⋅ W).
+Proof. done. Qed.
 
 Lemma subseteq_view_incl V W : (V ⊑ W) = (V ≼ W).
 Proof. done. Qed.
 
 Global Instance subseteq_view_assoc : Assoc (=) (join_view).
 Proof. apply _. Qed.
-
-(* Global Instance subseteq_view_transitive' : Transitive (subseteq_view).
-Proof.
-  intros V1 V2 V3. rewrite /subseteq_view.
-  intros H H'. rewrite -H'. rewrite assoc. rewrite H. done.
-Qed. *)
-
-(* Lemma view_lt (V W : view) : V ⊑ W ↔ ∃ V', V ⊔ V' = W.
-Proof.
-Admitted. *)
 
 Infix "!!0" := (λ m i, default 0 (max_nat_car <$> (m !! i))) (at level 80).
 
@@ -65,9 +48,6 @@ Proof.
     intros [?|[? [? (_ & ? & _)]]]; done.
 Qed.
 
-(* Definition view_to_ra (v : view) : view := (@id view). *)
-  (* MaxNat <$> v. *)
-
 Global Instance view_core_id (v : view) : CoreId v.
 Proof. apply _. Qed.
 
@@ -79,48 +59,12 @@ Proof. Admitted.
 Lemma view_valid V : ✓ V.
 Proof. intros k. case (V !! k); done. Qed.
 
-(* Lemma view_to_ra_injective V U : view_to_ra V ≡ view_to_ra U → V = U.
-Proof.
-  intros H.
-  apply map_eq.
-  intros ℓ.
-  pose proof (H ℓ) as Heq%leibniz_equiv.
-  rewrite !lookup_fmap in Heq.
-  destruct (V !! ℓ), (U !! ℓ); try done.
-  by inversion Heq.
-Qed. *)
+Lemma view_insert_le V ℓ t :
+  (V !!0 ℓ) ≤ t → V ⊑ <[ℓ := MaxNat t]>V.
+Proof. Admitted.
 
-(* Lemma view_to_ra_surjective U : ∃ V, view_to_ra V ≡ U.
+Lemma view_insert_op V ℓ t :
+  (V !!0 ℓ) ≤ t → (V ⊔ {[ℓ := MaxNat t]}) = (<[ℓ := MaxNat t]> V).
 Proof.
-  exists (max_nat_car <$> U). intros K.
-  rewrite /view_to_ra. rewrite !lookup_fmap.
-  destruct (U !! K) as [[n]|] eqn:Eq; rewrite Eq; done.
-Qed. *)
-
-(* Check view_to_ra_surjective. *)
-
-(* Lemma view_to_ra_op V W : view_to_ra V ⋅ view_to_ra W = view_to_ra (V ⊔ W).
-Proof.
-  apply leibniz_equiv.
-  intros K.
-  rewrite /view_to_ra.
-  rewrite lookup_op.
-  rewrite !lookup_fmap.
-  rewrite lookup_union_with.
-  destruct (V !! K), (W !! K); done.
-Qed. *)
-
-(* NOTE: The other direction should hold as well. *)
-(* Lemma view_to_ra_incl V W : view_to_ra V ≼ view_to_ra W → V ⊑ W.
-Proof.
-  intros [U Heq%leibniz_equiv].
-  (* apply view_to_ra_surjective in U. *) (* Why does this now work? *)
-  pose proof (view_to_ra_surjective U) as [V' Heq'%leibniz_equiv].
-  rewrite <- Heq' in Heq.
-  apply view_lt.
-  rewrite view_to_ra_op in Heq.
-  eexists _.
-  apply view_to_ra_injective.
-  rewrite Heq.
-  done.
-Qed. *)
+  intros look.
+Admitted.
